theories/typing.v
@@ -7,22 +7,26 @@ Require Import RecordUpdate.RecordUpdate.
 
 Require Import RichWasm.syntax.
 
-Record module_ctx :=
-  { mc_globals : list (mutability * type);
-    mc_table : list function_type }.
+Record module_ctx {K : Type} :=
+  { mc_globals : list (mutability * type K);
+    mc_table : list (function_type K) }.
 
-Definition local_ctx := list type.
+Arguments module_ctx : clear implicits.
 
-Record function_ctx :=
-  { fc_result_type : list type;
-    fc_labels : list (list type * local_ctx);
+Definition local_ctx (K : Type) := list (type K).
+
+Record function_ctx {K : Type} :=
+  { fc_result_type : list (type K);
+    fc_labels : list (list (type K) * local_ctx K);
     fc_location_vars : nat;
     fc_own_vars : nat;
     fc_rep_vars : nat;
     fc_size_vars : nat;
     fc_type_vars : list kind }.
 
-Definition fc_empty : function_ctx :=
+Arguments function_ctx : clear implicits.
+
+Definition fc_empty {K : Type} : function_ctx K :=
   {| fc_result_type := [];
      fc_labels := [];
      fc_location_vars := 0;
@@ -31,28 +35,28 @@ Definition fc_empty : function_ctx :=
      fc_size_vars := 0;
      fc_type_vars := [] |}.
 
-Global Instance eta_function_ctx : Settable _ :=
-  settable! Build_function_ctx
+Global Instance eta_function_ctx {K : Type} : Settable _ :=
+  settable! (@Build_function_ctx K)
   <fc_result_type; fc_labels; fc_location_vars; fc_own_vars; fc_rep_vars; fc_size_vars;
    fc_type_vars>.
 
-Definition update_locals (le : local_effect) (L : local_ctx) : local_ctx :=
+Definition update_locals {K : Type} (le : local_effect K) (L : local_ctx K) : local_ctx K :=
   fold_left (fun acc '(i, τ) => <[ i := τ ]> acc) le L.
 
-Inductive rep_ok : function_ctx -> representation -> Prop :=
-| VarROK (F : function_ctx) (r : variable) :
+Inductive rep_ok {K : Type} : function_ctx K -> representation -> Prop :=
+| VarROK (F : function_ctx K) (r : variable) :
   r < F.(fc_rep_vars) -> rep_ok F (VarR r)
-| SumROK (F : function_ctx) (ρs : list representation) :
+| SumROK (F : function_ctx K) (ρs : list representation) :
   Forall (rep_ok F) ρs -> rep_ok F (SumR ρs)
-| ProdROK (F : function_ctx) (ρs : list representation) :
+| ProdROK (F : function_ctx K) (ρs : list representation) :
   Forall (rep_ok F) ρs -> rep_ok F (ProdR ρs)
-| PrimROK (F : function_ctx) (ι : primitive_rep) :
+| PrimROK (F : function_ctx K) (ι : primitive_rep) :
   rep_ok F (PrimR ι).
 
-Inductive kind_ok : function_ctx -> kind -> Prop :=
-| VALTYPEOK (F : function_ctx) (ρ : representation) (γ : linearity) :
+Inductive kind_ok {K : Type} : function_ctx K -> kind -> Prop :=
+| VALTYPEOK (F : function_ctx K) (ρ : representation) (γ : linearity) :
   rep_ok F ρ -> kind_ok F (VALTYPE ρ γ)
-| MEMTYPEOK (F : function_ctx) (ζ : sizity) (μ : memory) (γ : linearity) :
+| MEMTYPEOK (F : function_ctx K) (ζ : sizity) (μ : memory) (γ : linearity) :
   kind_ok F (MEMTYPE ζ μ γ).
 
 Inductive mono_rep : representation -> list primitive_rep -> Prop :=
@@ -83,7 +87,7 @@ Definition primitive_size (ι : primitive_rep) : nat :=
   | F64R => 2
   end.
 
-Inductive has_kind : function_ctx -> type -> kind -> Prop :=
+Inductive has_kind : function_ctx kind -> type kind -> kind -> Prop :=
 | KSubValLin F τ ρ :
   has_kind F τ (VALTYPE ρ Unr) ->
   has_kind F τ (VALTYPE ρ Lin)
@@ -96,84 +100,102 @@ Inductive has_kind : function_ctx -> type -> kind -> Prop :=
 | KVar F t κ :
   F.(fc_type_vars) !! t = Some κ ->
   kind_ok F κ ->
-  has_kind F (VarT t) κ
+  has_kind F (VarT κ t) κ
 | KI32 F :
-  has_kind F (NumT (IntT I32T)) (VALTYPE (PrimR I32R) Unr)
+  let κ := VALTYPE (PrimR I32R) Unr in
+  has_kind F (NumT κ (IntT I32T)) κ
 | KI64 F :
-  has_kind F (NumT (IntT I64T)) (VALTYPE (PrimR I64R) Unr)
+  let κ := VALTYPE (PrimR I64R) Unr in
+  has_kind F (NumT κ (IntT I64T)) κ
 | KF32 F :
-  has_kind F (NumT (FloatT F32T)) (VALTYPE (PrimR F32R) Unr)
+  let κ := VALTYPE (PrimR F32R) Unr in
+  has_kind F (NumT κ (FloatT F32T)) κ
 | KF64 F :
-  has_kind F (NumT (FloatT F64T)) (VALTYPE (PrimR F64R) Unr)
+  let κ := VALTYPE (PrimR F64R) Unr in
+  has_kind F (NumT κ (FloatT F64T)) κ
 | KSumVal F τs ρs γ :
   Forall2 (fun τ ρ => has_kind F τ (VALTYPE ρ γ)) τs ρs ->
-  has_kind F (SumT τs) (VALTYPE (SumR ρs) γ)
+  let κ := VALTYPE (SumR ρs) γ in
+  has_kind F (SumT κ τs) κ
 | KSumMem F τs ζs μ γ :
   Forall2 (fun τ ζ => has_kind F τ (MEMTYPE ζ μ γ)) τs ζs ->
-  has_kind F (SumT τs) (MEMTYPE Unsized μ γ)
+  let κ := MEMTYPE Unsized μ γ in
+  has_kind F (SumT κ τs) κ
 | KSumMemSized F τs σs μ γ :
   Forall2 (fun τ σ => has_kind F τ (MEMTYPE (Sized σ) μ γ)) τs σs ->
-  has_kind F (SumT τs) (MEMTYPE (Sized (SumS σs)) μ γ)
+  let κ := MEMTYPE (Sized (SumS σs)) μ γ in
+  has_kind F (SumT κ τs) κ
 | KProdVal F τs ρs γ :
   Forall2 (fun τ ρ => has_kind F τ (VALTYPE ρ γ)) τs ρs ->
-  has_kind F (ProdT τs) (VALTYPE (ProdR ρs) γ)
+  let κ := VALTYPE (ProdR ρs) γ in
+  has_kind F (ProdT κ τs) κ
 | KProdMem F τs τn σs ζ μ γ :
+  (* TODO: Maybe the requirement that all preceding components are sized should be in the typing
+           rule for load instead. *)
   Forall2 (fun τ σ => has_kind F τ (MEMTYPE (Sized σ) μ γ)) τs σs ->
   has_kind F τn (MEMTYPE ζ μ γ) ->
-  has_kind F (ProdT (τs ++ [τn])) (MEMTYPE Unsized μ γ)
+  let κ := MEMTYPE Unsized μ γ in
+  has_kind F (ProdT κ (τs ++ [τn])) κ
 | KProdMemSized F τs σs μ γ :
   Forall2 (fun τ σ => has_kind F τ (MEMTYPE (Sized σ) μ γ)) τs σs ->
-  has_kind F (ProdT τs) (MEMTYPE (Sized (ProdS σs)) μ γ)
+  let κ := MEMTYPE (Sized (ProdS σs)) μ γ in
+  has_kind F (ProdT κ τs) κ
 | KArray F τ σ μ :
   has_kind F τ (MEMTYPE (Sized σ) μ Unr) ->
-  has_kind F (ArrayT τ) (MEMTYPE Unsized μ Unr)
+  let κ := MEMTYPE Unsized μ Unr in
+  has_kind F (ArrayT κ τ) κ
 | KExMem F τ κ :
   has_kind (set fc_own_vars S F) τ κ ->
-  has_kind F (ExT QMem τ) κ
+  has_kind F (ExT κ QMem τ) κ
 | KExRep F τ κ :
   has_kind (set fc_rep_vars S F) τ κ ->
-  has_kind F (ExT QRep τ) κ
+  has_kind F (ExT κ QRep τ) κ
 | KExSize F τ κ :
   has_kind (set fc_size_vars S F) τ κ ->
-  has_kind F (ExT QSize τ) κ
+  has_kind F (ExT κ QSize τ) κ
 | KExType F τ κ0 κ :
   has_kind (set fc_type_vars (cons κ0) F) τ κ ->
-  has_kind F (ExT (QType κ0) τ) κ
+  has_kind F (ExT κ (QType κ0) τ) κ
 | KRec F τ κ :
   (* TODO: Unfold. *)
   has_kind F τ κ ->
-  has_kind F (RecT τ) κ
+  has_kind F (RecT κ τ) κ
 | KRef F ω τ ζ μ γ :
   has_kind F τ (MEMTYPE ζ μ γ) ->
-  has_kind F (RefT ω τ) (VALTYPE (PrimR PtrR) Lin)
+  let κ := VALTYPE (PrimR PtrR) Lin in
+  has_kind F (RefT κ ω τ) κ
 | KCodeRef F ϕ :
-  has_kind F (CodeRefT ϕ) (VALTYPE (PrimR I32R) Unr)
+  let κ := VALTYPE (PrimR I32R) Unr in
+  has_kind F (CodeRefT κ ϕ) κ
 | KRep F ρ0 ρ τ γ :
   has_kind F τ (VALTYPE ρ0 γ) ->
-  has_kind F (RepT ρ τ) (VALTYPE ρ γ)
+  let κ := VALTYPE ρ γ in
+  has_kind F (RepT κ ρ τ) κ
 | KPad F σ0 σ τ μ γ :
   has_kind F τ (MEMTYPE (Sized σ0) μ γ) ->
-  has_kind F (PadT σ τ) (MEMTYPE (Sized σ) μ γ)
+  let κ := MEMTYPE (Sized σ) μ γ in
+  has_kind F (PadT κ σ τ) κ
 | KSer F τ ρ μ γ :
   has_kind F τ (VALTYPE ρ γ) ->
-  has_kind F (SerT τ) (MEMTYPE (Sized (RepS ρ)) μ γ).
+  let κ := MEMTYPE (Sized (RepS ρ)) μ γ in
+  has_kind F (SerT κ τ) κ.
 
-Inductive has_rep : function_ctx -> type -> representation -> Prop :=
-| RepVALTYPE (F : function_ctx) (τ : type) (ρ : representation) (γ : linearity) :
+Inductive has_rep : function_ctx kind -> type kind -> representation -> Prop :=
+| RepVALTYPE (F : function_ctx kind) (τ : type kind) (ρ : representation) (γ : linearity) :
   has_kind F τ (VALTYPE ρ γ) ->
   has_rep F τ ρ.
 
-Inductive mono_sized : function_ctx -> type -> Prop :=
-| MonoSized (F : function_ctx) (τ : type) (ρ : representation) (ιs : list primitive_rep) :
+Inductive mono_sized : function_ctx kind -> type kind -> Prop :=
+| MonoSized (F : function_ctx kind) (τ : type kind) (ρ : representation) (ιs : list primitive_rep) :
   has_rep F τ ρ ->
   mono_rep ρ ιs ->
   mono_sized F τ.
 
-Inductive is_unrestricted : function_ctx -> type -> Prop :=
-| UnrVALTYPE (F : function_ctx) (τ : type) (ρ : representation) :
+Inductive is_unrestricted : function_ctx kind -> type kind -> Prop :=
+| UnrVALTYPE (F : function_ctx kind) (τ : type kind) (ρ : representation) :
   has_kind F τ (VALTYPE ρ Unr) ->
   is_unrestricted F τ
-| UnrMEMTYPE (F : function_ctx) (τ : type) (ζ : sizity) (μ : memory) :
+| UnrMEMTYPE (F : function_ctx kind) (τ : type kind) (ζ : sizity) (μ : memory) :
   has_kind F τ (MEMTYPE ζ μ Unr) ->
   is_unrestricted F τ.
 
@@ -188,51 +210,51 @@ Inductive convertible_to : list primitive_rep -> list primitive_rep -> Prop :=
 | ConvertPtr ιs1 ιs2 :
   convertible_to (PtrR :: ιs1) (PtrR :: ιs2).
 
-Inductive path_to : path -> type -> list type -> type -> Prop :=
+Inductive path_to {K : Type} : path -> type K -> list (type K) -> type K -> Prop :=
 | PathToNil τ :
   path_to [] τ [] τ
-| PathToRep π ρ τ τs τ' :
+| PathToRep ann π ρ τ τs τ' :
   path_to π τ τs τ' ->
-  path_to (PCUnwrap :: π) (RepT ρ τ) τs τ'
-| PathToPad π σ τ τs τ' :
+  path_to (PCUnwrap :: π) (RepT ann ρ τ) τs τ'
+| PathToPad ann π σ τ τs τ' :
   path_to (PCUnwrap :: π) τ τs τ' ->
-  path_to π (PadT σ τ) τs τ'
-| PathToSer π τ τs τ' :
+  path_to π (PadT ann σ τ) τs τ'
+| PathToSer ann π τ τs τ' :
   path_to π τ τs τ' ->
-  path_to (PCUnwrap :: π) (SerT τ) τs τ'
-| PathToEx π δ τ τs τ' :
+  path_to (PCUnwrap :: π) (SerT ann τ) τs τ'
+| PathToEx ann π δ τ τs τ' :
   path_to π τ τs τ' ->
-  path_to (PCUnwrap :: π) (ExT δ τ) τs τ'
-| PathToRec π τ τs τ' :
+  path_to (PCUnwrap :: π) (ExT ann δ τ) τs τ'
+| PathToRec ann π τ τs τ' :
   path_to π τ τs τ' ->
-  path_to (PCUnwrap :: π) (RecT τ) τs τ'
-| PathToProd n π τs τs0 τs' τ τ0 :
+  path_to (PCUnwrap :: π) (RecT ann τ) τs τ'
+| PathToProd ann n π τs τs0 τs' τ τ0 :
   length τs0 = n ->
   path_to π τ0 τs τ ->
-  path_to (PCProj n :: π) (ProdT (τs0 ++ τ0 :: τs')) (τs0 ++ τs) τ.
+  path_to (PCProj n :: π) (ProdT ann (τs0 ++ τ0 :: τs')) (τs0 ++ τs) τ.
 
-Inductive update_at : path -> type -> type -> type -> type -> Prop :=
+Inductive update_at {K : Type} : path -> type K -> type K -> type K -> type K -> Prop :=
 | UpdateAtNil τ τ' :
   update_at [] τ τ τ' τ'
-| UpdateAtRep π ρ τ τ' τ__π τ__π' :
+| UpdateAtRep ann π ρ τ τ' τ__π τ__π' :
   update_at π τ τ__π τ' τ__π' ->
-  update_at (PCUnwrap :: π) (RepT ρ τ) τ__π (RepT ρ τ') τ__π'
-| UpdateAtPad π σ τ τ' τ__π τ__π' :
+  update_at (PCUnwrap :: π) (RepT ann ρ τ) τ__π (RepT ann ρ τ') τ__π'
+| UpdateAtPad ann π σ τ τ' τ__π τ__π' :
   update_at π τ τ__π τ' τ__π' ->
-  update_at (PCUnwrap :: π) (PadT σ τ) τ__π (PadT σ τ') τ__π'
-| UpdateAtSer π τ τ' τ__π τ__π' :
+  update_at (PCUnwrap :: π) (PadT ann σ τ) τ__π (PadT ann σ τ') τ__π'
+| UpdateAtSer ann π τ τ' τ__π τ__π' :
   update_at π τ τ__π τ' τ__π' ->
-  update_at (PCUnwrap :: π) (SerT τ) τ__π (SerT τ') τ__π'
-| UpdateAtEx π δ τ τ' τ__π τ__π'  :
+  update_at (PCUnwrap :: π) (SerT ann τ) τ__π (SerT ann τ') τ__π'
+| UpdateAtEx ann π δ τ τ' τ__π τ__π'  :
   update_at π τ τ__π τ' τ__π' ->
-  update_at (PCUnwrap :: π) (ExT δ τ) τ__π (ExT δ τ') τ__π'
-| UpdateAtRec π τ τ' τ__π τ__π' :
+  update_at (PCUnwrap :: π) (ExT ann δ τ) τ__π (ExT ann δ τ') τ__π'
+| UpdateAtRec ann π τ τ' τ__π τ__π' :
   update_at π τ τ__π τ' τ__π' ->
-  update_at (PCUnwrap :: π) (RecT τ) τ__π (RecT τ') τ__π'
-| UpdateAtProd π τ τ' τ__π τ__π' τs τs' n :
+  update_at (PCUnwrap :: π) (RecT ann τ) τ__π (RecT ann τ') τ__π'
+| UpdateAtProd ann π τ τ' τ__π τ__π' τs τs' n :
   length τs = n ->
   update_at π τ τ__π τ' τ__π' ->
-  update_at (PCProj n :: π) (ProdT (τs ++ τ :: τs')) τ__π (ProdT (τs ++ τ' :: τs')) τ__π'.
+  update_at (PCProj n :: π) (ProdT ann (τs ++ τ :: τs')) τ__π (ProdT ann (τs ++ τ' :: τs')) τ__π'.
 
 Inductive mono_size : size -> nat -> Prop :=
 | MonoSizeSum σs ns :
@@ -247,115 +269,152 @@ Inductive mono_size : size -> nat -> Prop :=
 | MonoSizeConst n :
   mono_size (ConstS n) n.
 
-Inductive stores_as : function_ctx -> type -> type -> Prop :=
-| SASer F τ :
-  stores_as F τ (SerT τ)
-| SAPad F τ τ' ρ ιs σ n :
+Inductive stores_as : function_ctx kind -> type kind -> type kind -> Prop :=
+| SASer F κ τ :
+  stores_as F τ (SerT κ τ)
+| SAPad F κ τ τ' ρ ιs σ n :
   has_rep F τ ρ ->
   mono_rep ρ ιs ->
   mono_size σ n ->
   list_sum (map primitive_size ιs) <= n ->
   stores_as F τ τ' ->
-  stores_as F τ (PadT σ τ')
-| SAProd F τs τs' :
+  stores_as F τ (PadT κ σ τ')
+| SAProd F κ τs τs' :
   Forall2 (stores_as F) τs τs' ->
-  stores_as F (ProdT τs) (ProdT τs').
+  stores_as F (ProdT κ τs) (ProdT κ τs').
 
 (* Handy name for the converse of stores_as. *)
 Definition loads_as F τ τ' := stores_as F τ' τ.
 
-Inductive module_ctx_ok : module_ctx -> Prop :=
-| MC_OK (gs : list (mutability * type)) ts :
+Inductive module_ctx_ok : module_ctx kind -> Prop :=
+| MC_OK (gs : list (mutability * type kind)) ts :
   Forall (fun '(_, τ) => is_unrestricted fc_empty τ) gs ->
   module_ctx_ok {| mc_globals := gs; mc_table := ts |}.
 
 (* TODO *)
-Inductive num_instr_has_type : num_instr -> arrow_type -> Prop :=.
+Inductive num_instr_has_type : num_instr -> arrow_type kind -> Prop :=.
 
-Inductive instr_has_type {A : Type} :
-  module_ctx -> function_ctx -> local_ctx -> instr A -> arrow_type -> local_ctx -> Prop :=
-| TNop M F L ann :
-  instr_has_type M F L (INop ann) (ArrowT [] []) L
-| TDrop M F L ann τ :
+Inductive instr_has_type :
+  module_ctx kind ->
+  function_ctx kind ->
+  local_ctx kind ->
+  instr (arrow_type kind) kind ->
+  arrow_type kind ->
+  local_ctx kind ->
+  Prop :=
+| TNop M F L :
+  let χ := ArrowT [] [] in
+  instr_has_type M F L (INop χ) χ L
+| TDrop M F L τ :
   is_unrestricted F τ ->
-  instr_has_type M F L (IDrop ann) (ArrowT [τ] []) L
-| TUnreachable M F L L' ann τs1 τs2 le :
-  L' = update_locals le L ->
-  instr_has_type M F L (IUnreachable ann) (ArrowT τs1 τs2) L
-| TNum M F L ann en χ :
+  let χ := ArrowT [τ] [] in
+  instr_has_type M F L (IDrop χ) χ L
+| TUnreachable M F L τs1 τs2 le :
+  let L' := update_locals le L in
+  let χ := ArrowT τs1 τs2 in
+  instr_has_type M F L (IUnreachable χ) χ L'
+| TNum M F L en χ :
   num_instr_has_type en χ ->
-  instr_has_type M F L (INum ann en) χ L
-| TNumConst M F L ann ν n :
-  instr_has_type M F L (INumConst ann ν n) (ArrowT [] [NumT ν]) L
-| TBlock M F F' L L' ann τs1 τs2 le es :
-  F' = set fc_labels (cons (τs2, L')) F ->
-  L' = update_locals le L ->
-  expr_has_type M F L es (ArrowT τs1 τs2) L' ->
-  instr_has_type M F L (IBlock ann (ArrowT τs1 τs2) le es) (ArrowT τs1 τs2) L'
-| TLoop M F F' L ann τs1 τs2 es :
-  F' = set fc_labels (cons (τs1, L)) F ->
-  expr_has_type M F L es (ArrowT τs1 τs2) L ->
-  instr_has_type M F L (ILoop ann (ArrowT τs1 τs2) es) (ArrowT τs1 τs2) L
-| TIte M F L L' ann χ le es1 es2 :
-  L' = update_locals le L ->
+  instr_has_type M F L (INum χ en) χ L
+| TNumConst M F L κ ν n :
+  has_kind F (NumT κ ν) κ ->
+  let χ := ArrowT [] [NumT κ ν] in
+  instr_has_type M F L (INumConst χ ν n) χ L
+| TBlock M F L τs1 τs2 le es :
+  let L' := update_locals le L in
+  let F' := set fc_labels (cons (τs2, L')) F in
+  let χ := ArrowT τs1 τs2 in
+  expr_has_type M F' L es χ L' ->
+  instr_has_type M F L (IBlock χ (ArrowT τs1 τs2) le es) χ L'
+| TLoop M F L τs1 τs2 es :
+  let F' := set fc_labels (cons (τs1, L)) F in
+  let χ := ArrowT τs1 τs2 in
+  expr_has_type M F' L es χ L ->
+  instr_has_type M F L (ILoop χ χ es) χ L
+| TIte M F L χ le es1 es2 :
+  let L' := update_locals le L in
   expr_has_type M F L es1 χ L' ->
   expr_has_type M F L es2 χ L' ->
-  instr_has_type M F L (IIte ann χ le es1 es2) χ L'
-| TBr M F L L' ann n τs τs1 τs2 le :
-  L' = update_locals le L ->
+  instr_has_type M F L (IIte χ χ le es1 es2) χ L'
+| TBr M F L n τs τs1 τs2 le :
   F.(fc_labels) !! n = Some (τs, L) ->
   Forall (is_unrestricted F) τs1 ->
-  instr_has_type M F L (IBr ann n) (ArrowT (τs1 ++ τs) τs2) L'
-| TBrIf M F L ann n τs :
+  let χ := ArrowT (τs1 ++ τs) τs2 in
+  let L' := update_locals le L in
+  instr_has_type M F L (IBr χ n) χ L'
+| TBrIf M F L n τs κ :
   F.(fc_labels) !! n = Some (τs, L) ->
-  instr_has_type M F L (IBrIf ann n) (ArrowT (τs ++ [NumT (IntT I32T)]) τs) L
-| TBrTable M F L L' ann ns n τs τs1 τs2 :
+  let τ := NumT κ (IntT I32T) in
+  has_kind F τ κ ->
+  let χ := ArrowT (τs ++ [τ]) τs in
+  instr_has_type M F L (IBrIf χ n) χ L
+| TBrTable M F L L' ns n τs τs1 τs2 κ :
   Forall (fun i => F.(fc_labels) !! i = Some (τs, L)) (n :: ns) ->
   Forall (is_unrestricted F) τs1 ->
-  instr_has_type M F L (IBrTable ann ns n) (ArrowT (τs1 ++ τs ++ [NumT (IntT I32T)]) τs2) L'
-| TReturn M F L L' ann le τs τs1 τs2 :
+  let τ := NumT κ (IntT I32T) in
+  has_kind F τ κ ->
+  let χ := ArrowT (τs1 ++ τs ++ [τ]) τs2 in
+  instr_has_type M F L (IBrTable χ ns n) χ L'
+| TReturn M F L le τs τs1 τs2 :
   F.(fc_result_type) = τs ->
-  L' = update_locals le L ->
   Forall (is_unrestricted F) τs1 ->
-  instr_has_type M F L (IReturn ann) (ArrowT (τs1 ++ τs) τs2) L'
-| TLocalGet M F L L' ann n τ ρ :
+  let L' := update_locals le L in
+  let χ := ArrowT (τs1 ++ τs) τs2 in
+  instr_has_type M F L (IReturn χ) χ L'
+| TLocalGet M F L n τ ρ κ0 κ :
   L !! n = Some τ ->
   has_rep F τ ρ ->
-  L' = <[ n := RepT ρ (ProdT []) ]> L ->
-  instr_has_type M F L (ILocalGet ann n) (ArrowT [] [τ]) L'
-| TLocalGetUnr M F L ann n τ :
+  let τ' := RepT κ ρ (ProdT κ0 []) in
+  has_kind F τ' κ ->
+  let L' := <[ n := τ' ]> L in
+  let χ := ArrowT [] [τ] in
+  instr_has_type M F L (ILocalGet χ n) χ L'
+| TLocalGetUnr M F L n τ :
   L !! n = Some τ ->
   is_unrestricted F τ ->
-  instr_has_type M F L (ILocalGet ann n) (ArrowT [] [τ]) L
-| TLocalSet M F L L' ann n τ τ' ρ :
-  L' = <[ n := τ' ]> L ->
+  let χ := ArrowT [] [τ] in
+  instr_has_type M F L (ILocalGet χ n) χ L
+| TLocalSet M F L n τ τ' ρ :
   L !! n = Some τ ->
   is_unrestricted F τ ->
   has_rep F τ ρ ->
   has_rep F τ' ρ ->
-  instr_has_type M F L (ILocalSet ann n) (ArrowT [τ'] []) L'
-| TGlobalGet M F L ann n m τ :
+  let L' := <[ n := τ' ]> L in
+  let χ := ArrowT [τ'] [] in
+  instr_has_type M F L (ILocalSet χ n) χ L'
+| TGlobalGet M F L n m τ :
   M.(mc_globals) !! n = Some (m, τ) ->
-  instr_has_type M F L (IGlobalGet ann n) (ArrowT [] [τ]) L
-| TGlobalSet M F L ann n m τ :
+  let χ := ArrowT [] [τ] in
+  instr_has_type M F L (IGlobalGet χ n) χ L
+| TGlobalSet M F L n m τ :
   M.(mc_globals) !! n = Some (m, τ) ->
-  instr_has_type M F L (IGlobalSet ann n) (ArrowT [τ] []) L
-| TCodeRef M F L ann n ϕ :
+  let χ := ArrowT [τ] [] in
+  instr_has_type M F L (IGlobalSet χ n) χ L
+| TCodeRef M F L n ϕ κ :
   (mc_table M) !! n = Some ϕ ->
-  instr_has_type M F L (ICodeRef ann n) (ArrowT [] [CodeRefT ϕ]) L
+  let τ := CodeRefT κ ϕ in
+  has_kind F τ κ ->
+  let χ := ArrowT [] [τ] in
+  instr_has_type M F L (ICodeRef χ n) χ L
 (*
 | TCall M F L ann n ixs :
   instr_has_type M F L (ICall ann n ixs) (ArrowT [] []) L
 | TCallIndirect M F L ann ixs :
   instr_has_type M F L (ICallIndirect ann ixs) (ArrowT [] []) L
 *)
-| TGroup M F L ann n τs ρs γ :
+| TGroup M F L n κ τs ρs γ :
   length τs = n ->
   Forall2 (λ τ ρ, has_kind F τ (VALTYPE ρ γ)) τs ρs ->
-  instr_has_type M F L (IGroup ann n) (ArrowT τs [ProdT τs]) L
-| TUngroup M F L ann τs ρ γ :
-  has_kind F (ProdT τs) (VALTYPE ρ γ) ->
-  instr_has_type M F L (IUngroup ann) (ArrowT [ProdT τs] τs) L
+  let τ := ProdT κ τs in
+  has_kind F τ κ ->
+  let χ := ArrowT τs [τ] in
+  instr_has_type M F L (IGroup χ n) χ L
+| TUngroup M F L τs ρ γ :
+  let κ := VALTYPE ρ γ in
+  let τ := ProdT κ τs in
+  has_kind F τ κ ->
+  let χ := ArrowT [τ] τs in
+  instr_has_type M F L (IUngroup χ) χ L
 (* These require setting up substitution.
 | TFold M F L ann τ :
   instr_has_type M F L (IFold ann τ) (ArrowT [] []) L
@@ -366,64 +425,106 @@ Inductive instr_has_type {A : Type} :
 | TUnpack M F L ann χ le es :
   instr_has_type M F L (IUnpack ann χ le es) (ArrowT [] []) L
 *)
-| TWrap M F L ann ρ0 ρ ιs0 ιs τ :
+| TWrap M F L ρ0 ρ ιs0 ιs τ0 κ :
   mono_rep ρ0 ιs0 ->
   mono_rep ρ ιs ->
   convertible_to ιs0 ιs ->
-  instr_has_type M F L (IWrap ann) (ArrowT [τ] [RepT ρ τ]) L
-| TUnwrap M F L ann ρ0 ρ ιs0 ιs τ :
+  let τ := RepT κ ρ τ0 in
+  has_kind F τ κ ->
+  let χ := ArrowT [τ0] [τ] in
+  instr_has_type M F L (IWrap χ) χ L
+| TUnwrap M F L ρ0 ρ ιs0 ιs τ0 κ :
   mono_rep ρ0 ιs0 ->
   mono_rep ρ ιs ->
   convertible_to ιs0 ιs ->
-  instr_has_type M F L (IUnwrap ann) (ArrowT [RepT ρ τ] [τ]) L
-| TRefNew M F L ann ω τ τ' :
-  stores_as F τ τ' ->
-  instr_has_type M F L (IRefNew ann ω) (ArrowT [τ] [RefT ω τ']) L
-| TRefFree M F L ann τ :
-  is_unrestricted F τ ->
-  instr_has_type M F L (IRefFree ann) (ArrowT [RefT MemMM τ] []) L
-| TRefDup M F L ann τ :
-  instr_has_type M F L (IRefDup ann) (ArrowT [RefT MemGC τ] [RefT MemGC τ; RefT MemGC τ]) L
-| TRefDrop M F L ann τ :
-  instr_has_type M F L (IRefDrop ann) (ArrowT [RefT MemGC τ] []) L
-| TRefLoad M F L ann π μ τ τs__off τ' ρ ιs :
-  path_to π τ τs__off τ' ->
+  let τ := RepT κ ρ τ0 in
+  has_kind F τ κ ->
+  let χ := ArrowT [τ] [τ0] in
+  instr_has_type M F L (IUnwrap χ) χ L
+| TRefNew M F L μ τ0 τ0' κ :
+  stores_as F τ0 τ0' ->
+  let τ := RefT κ μ τ0' in
+  has_kind F τ κ ->
+  let χ := ArrowT [τ0] [τ] in
+  instr_has_type M F L (IRefNew χ μ) χ L
+| TRefFree M F L τ0 κ :
+  is_unrestricted F τ0 ->
+  let τ := RefT κ MemMM τ0 in
+  has_kind F τ κ ->
+  let χ := ArrowT [τ] [] in
+  instr_has_type M F L (IRefFree χ) χ L
+| TRefDup M F L τ0 κ :
+  let τ := RefT κ MemGC τ0 in
+  has_kind F τ κ ->
+  let χ := ArrowT [τ] [τ; τ] in
+  instr_has_type M F L (IRefDup χ) χ L
+| TRefDrop M F L τ0 κ :
+  let τ := RefT κ MemGC τ0 in
+  has_kind F τ κ ->
+  let χ := ArrowT [τ] [] in
+  instr_has_type M F L (IRefDrop χ) χ L
+| TRefLoad M F L π μ τ0 τs__off τ0' ρ ιs κ :
+  path_to π τ0 τs__off τ0' ->
   Forall (mono_sized F) τs__off ->
-  has_kind F τ' (VALTYPE ρ Unr) ->
+  has_kind F τ0' (VALTYPE ρ Unr) ->
   mono_rep ρ ιs ->
-  instr_has_type M F L (IRefLoad ann π) (ArrowT [RefT μ τ] [RefT μ τ; τ']) L
-| TRefStore M F L ann π μ τ τs τᵥ τ__π :
-  path_to π τ τs τ__π ->
+  let τ := RefT κ μ τ0 in
+  has_kind F τ κ ->
+  let χ := ArrowT [τ] [τ; τ0'] in
+  instr_has_type M F L (IRefLoad χ π) χ L
+| TRefStore M F L π μ τ0 τs τᵥ τ__π κ :
+  path_to π τ0 τs τ__π ->
   stores_as F τᵥ τ__π ->
   is_unrestricted F τ__π ->
-  instr_has_type M F L (IRefStore ann π) (ArrowT [RefT μ τ; τᵥ] [RefT μ τ]) L
-| TRefStoreUniq M F L ann π μ τ τ' τᵥ τᵥ' τₘ τₘ' σ σ' γ n :
+  let τ := RefT κ μ τ0 in
+  has_kind F τ κ ->
+  let χ := ArrowT [τ; τᵥ] [τ] in
+  instr_has_type M F L (IRefStore χ π) χ L
+| TRefStoreUniq M F L ann π μ τ0 τ0' τᵥ τᵥ' τₘ τₘ' κ κ' σ σ' γ n :
   stores_as F τᵥ τₘ' ->
-  update_at π τ τₘ τ' τₘ' ->
+  update_at π τ0 τₘ τ0' τₘ' ->
   has_kind F τₘ (MEMTYPE (Sized σ) μ Unr) ->
   has_kind F τₘ' (MEMTYPE (Sized σ') μ γ) ->
   mono_size σ n ->
   mono_size σ' n ->
-  instr_has_type M F L (IRefStore ann π) (ArrowT [RefT MemMM τ; τᵥ'] [RefT MemMM τ']) L
-| TRefSwap M F L ann π γ ρ ιs ω τ τᵥ τₘ τs__off :
+  let τ := RefT κ MemMM τ0 in
+  let τ' := RefT κ' MemMM τ0' in
+  has_kind F τ κ ->
+  has_kind F τ' κ' ->
+  instr_has_type M F L (IRefStore ann π) (ArrowT [τ; τᵥ'] [τ']) L
+| TRefSwap M F L π γ ρ ιs μ τ0 τᵥ τₘ τs__off κ :
   has_kind F τᵥ (VALTYPE ρ γ) ->
   mono_rep ρ ιs ->
-  path_to π τ τs__off τₘ ->
+  path_to π τ0 τs__off τₘ ->
   loads_as F τᵥ τₘ ->
   Forall (mono_sized F) τs__off ->
-  instr_has_type M F L (IRefSwap ann π) (ArrowT [RefT ω τ; τᵥ] [RefT ω τ; τᵥ]) L
-| TRefSwapUniq M F L ann π γ ρ ιs τ τ' τᵥ τᵥ' τₘ τₘ' τs__off :
+  let τ := RefT κ μ τ0 in
+  has_kind F τ κ ->
+  let χ := ArrowT [τ; τᵥ] [τ; τᵥ] in
+  instr_has_type M F L (IRefSwap χ π) χ L
+| TRefSwapUniq M F L π γ ρ ιs τ0 τ0' τᵥ τᵥ' τₘ τₘ' τs__off κ κ' :
   has_kind F τᵥ (VALTYPE ρ γ) ->
   mono_rep ρ ιs ->
-  path_to π τ τs__off τₘ ->
+  path_to π τ0 τs__off τₘ ->
   loads_as F τᵥ τₘ ->
   stores_as F τᵥ' τₘ' ->
-  update_at π τ τₘ τ' τₘ' ->
+  update_at π τ0 τₘ τ0' τₘ' ->
   Forall (mono_sized F) τs__off ->
-  instr_has_type M F L (IRefSwap ann π) (ArrowT [RefT MemMM τ; τᵥ'] [RefT MemMM τ'; τᵥ]) L
+  let τ := RefT κ MemMM τ0 in
+  let τ' := RefT κ' MemMM τ0' in
+  has_kind F τ κ ->
+  has_kind F τ' κ' ->
+  let χ := ArrowT [τ; τᵥ'] [τ'; τᵥ] in
+  instr_has_type M F L (IRefSwap χ π) χ L
 
-with expr_has_type {A : Type} :
-  module_ctx -> function_ctx -> local_ctx -> expr A -> arrow_type -> local_ctx -> Prop :=
+with expr_has_type :
+  module_ctx kind ->
+  function_ctx kind ->
+  local_ctx kind ->
+  expr (arrow_type kind) kind ->
+  arrow_type kind ->
+  local_ctx kind ->
+  Prop :=
 | TNil M F L :
   expr_has_type M F L [] (ArrowT [] []) L
 | TCons M F L1 L2 L3 e es τs1 τs2 τs3 :
